src/Bedrock/End2End/X25519/CachedMultiples.v
@@ -1,0 +1,337 @@
+Require Import bedrock2.Array.
+Require Import bedrock2.bottom_up_simpl.
+Require Import bedrock2.FE310CSemantics.
+Require Import bedrock2.Loops.
+Require Import bedrock2.Map.Separation.
+Require Import bedrock2.Map.SeparationLogic.
+Require Import bedrock2.NotationsCustomEntry.
+Require Import bedrock2.ProgramLogic.
+Require Import bedrock2.Scalars.
+Require Import bedrock2.Semantics.
+Require Import bedrock2.SepAutoArray.
+Require Import bedrock2.Syntax.
+Require Import bedrock2.WeakestPrecondition.
+Require Import bedrock2.WeakestPreconditionProperties.
+Require Import bedrock2.ZnWords.
+Require Import compiler.MMIO.
+Require Import compiler.Pipeline.
+Require Import compiler.Symbols.
+Require Import coqutil.Byte.
+Require Import coqutil.Map.Interface.
+Require Import coqutil.Map.OfListWord.
+From coqutil.Tactics Require Import Tactics letexists eabstract rdelta reference_to_string ident_of_string.
+Require Import coqutil.Word.Bitwidth32.
+Require Import coqutil.Word.Interface.
+Require Import coqutil.Word.Naive.
+From Coq Require Import Init.Byte.
+From Coq Require Import List.
+From Coq Require Import String.
+From Coq Require Import ZArith.
+Require Import Crypto.Arithmetic.PrimeFieldTheorems.
+Require Import Crypto.Bedrock.Field.Synthesis.New.UnsaturatedSolinas.
+Require Import Crypto.Bedrock.End2End.X25519.Field25519.
+Require Import Crypto.Bedrock.End2End.X25519.EdwardsXYZT. (* todo rename and move around properly, try to create a proper hierarchy of what needs what *)
+Require Import Crypto.Bedrock.Specs.Field.
+Require Import Crypto.Spec.Curve25519.
+Require Import Crypto.Util.Decidable.
+Require Import Crypto.Util.Tactics.DestructHead.
+Require Import Curves.Edwards.XYZT.Basic.
+Require Import Curves.Edwards.XYZT.Precomputed.
+Require Import Curves.Edwards.XYZT.Readdition.
+Require Import Lia.
+Require Crypto.Bedrock.Field.Synthesis.New.Signature.
+Local Open Scope string_scope.
+Local Open Scope Z_scope.
+Import LittleEndianList.
+Import ListNotations.
+Import ProgramLogic.Coercions.
+Import WeakestPrecondition.
+
+Local Existing Instance field_parameters.
+Local Existing Instance frep25519.
+Local Existing Instance frep25519_ok.
+
+(* Size of a field element in bytes. This is the same as computing eval in felem_size_bytes, but we want a notation instead of definition. *)
+Local Notation felem_size := 40.
+(* Size of a projective point in bytes. *)
+Local Notation pp_size := 200.
+(* Size of a cached point in bytes. *)
+Local Notation pc_size := 160.
+
+(* Notations help treat curve points like C structs. To avoid notation clashes, projective coordinates are capitalized. *)
+
+(* Member access notation for projective points: (X, Y, Z, Ta, Tb). *)
+Local Notation "A .X" := (A) (in custom bedrock_expr at level 2, left associativity, only parsing).
+Local Notation "A .Y" := (expr.op Syntax.bopname.add A (felem_size)) (in custom bedrock_expr at level 2, left associativity, only parsing).
+Local Notation "A .Z" := (expr.op Syntax.bopname.add A (felem_size + felem_size)) (in custom bedrock_expr at level 2, left associativity, only parsing).
+Local Notation "A .Ta" := (expr.op Syntax.bopname.add A (felem_size + felem_size + felem_size)) (in custom bedrock_expr at level 2, left associativity, only parsing).
+Local Notation "A .Tb" := (expr.op Syntax.bopname.add A (felem_size + felem_size + felem_size + felem_size)) (in custom bedrock_expr at level 2, left associativity, only parsing).
+
+(* Member access notation for cached points: (half_YmX, half_YpX, Z, Td). *)
+Local Notation "A .half_YmX" := (A) (in custom bedrock_expr at level 2, left associativity, only parsing).
+Local Notation "A .half_YpX" := (expr.op Syntax.bopname.add A (felem_size)) (in custom bedrock_expr at level 2, left associativity, only parsing).
+Local Notation "A .Z" := (expr.op Syntax.bopname.add A (felem_size + felem_size)) (in custom bedrock_expr at level 2, left associativity, only parsing).
+Local Notation "A .Td" := (expr.op Syntax.bopname.add A (felem_size + felem_size + felem_size)) (in custom bedrock_expr at level 2, left associativity, only parsing).
+
+(* Input is a projective point p, output is multiples of p as cached points, to be used for scalar multiplication. *)
+Definition cached_multiples := func! (p_ai, p_a, p_d) {
+  (* The first point is 0*A, so just zero. *)
+  stackalloc pp_size as zero;
+  zero_projective_point(zero);
+  to_cached(p_ai, zero, p_d);
+
+  (* The second point is 1*A.*)
+  to_cached(p_ai+$pc_size, p_a, p_d);
+
+  (* Helper array of normal points for double and add results, contains multiples of A. *)
+  stackalloc 8*pp_size as p_ai_uncached;
+  (* copy 1*A into the helper array at index 1. *)
+  copy_projective_point(p_ai_uncached+$pp_size, p_a);
+
+  (* Remaining points are generated in a loop. *)
+  i = $2;
+  stackalloc pp_size as temp;
+  while (i < $16) {
+    double(temp, p_ai_uncached+((i >> $1) * $pp_size)); (* Double (i/2)*A, now temp contains i*A. *)
+    to_cached(p_ai+(i*$pc_size), temp, p_d); (* copy temp to Ai *)
+    if (i < $8) {
+      (* Save i*A for later, at index i. *)
+      copy_projective_point(p_ai_uncached+(i*$pp_size), temp)
+    };
+    (* Now for the odd numbers, calculate (i+1)*A, store in temp. *)
+    readd(temp, p_a, p_ai+(i*$pc_size));
+    (* Store (i+1)*A in the result array. *)
+    to_cached(p_ai+((i+$1)*$pc_size), temp, p_d);
+    if (i < $7) {
+      (* Save (i+1)*A for later. *)
+      copy_projective_point(p_ai_uncached+((i+$1)*$pp_size), temp)
+    };
+    i = i + $2
+  }
+}.
+
+Section WithParameters.
+Context {two_lt_M: 2 < M_pos}.
+(* TODO: Can we provide actual values/proofs for these, rather than just sticking them in the context? *)
+Context {char_ge_3 : (@Ring.char_ge (F M_pos) Logic.eq F.zero F.one F.opp F.add F.sub F.mul (BinNat.N.succ_pos BinNat.N.two))}.
+Context {field:@Algebra.Hierarchy.field (F M_pos) Logic.eq F.zero F.one F.opp F.add F.sub F.mul F.inv F.div}.
+Context {a d: F M_pos}
+        {nonzero_a : a <> F.zero}
+        {square_a : exists sqrt_a, (F.mul sqrt_a sqrt_a) = a}
+        {nonsquare_d : forall x, (F.mul x x) <> d}.
+Context {a_eq_minus1:a = F.opp F.one} {twice_d} {k_eq_2d:twice_d = (F.add d d)} {nonzero_d: d<>F.zero}.
+
+(* Avoid unfolding deeper than necessary. *)
+Local Opaque F.to_Z word.rep word.wrap word.unsigned word.of_Z word.add feval.
+
+Local Notation "m =* P" := ((P%sep) m) (at level 70, only parsing).
+
+Local Notation FElem := (FElem(FieldRepresentation:=frep25519)).
+Local Notation felem_size_in_bytes := (felem_size_in_bytes(FieldRepresentation:=frep25519)).
+Local Notation bounded_by := (bounded_by(FieldRepresentation:=frep25519)).
+Local Notation word := (Naive.word 32).
+Local Notation felem := (felem(FieldRepresentation:=frep25519)).
+Local Notation point := (point(Feq:=Logic.eq)(Fzero:=F.zero)(Fadd:=F.add)(Fmul:=F.mul)(a:=a)(d:=d)).
+Local Notation cached := (cached(Fzero:=F.zero)(Fadd:=F.add)(Fmul:=F.mul)(a:=a)(d:=d)).
+Local Notation coordinates := (coordinates(Fzero:=F.zero)(Fadd:=F.add)(Fmul:=F.mul)(Feq:=Logic.eq)(a:=a)(d:=d)).
+Local Notation cached_coordinates := (cached_coordinates(Fzero:=F.zero)(Fadd:=F.add)(Fdiv:=F.div)(Fmul:=F.mul)(Fsub:=F.sub)(Feq:=Logic.eq)(a:=a)(d:=d)).
+Local Notation m1_prep :=
+  (m1_prep(F:=F M_pos)(Feq:=Logic.eq)(Fzero:=F.zero)(Fone:=F.one)
+                  (Fopp:=F.opp)(Fadd:=F.add)(Fsub:=F.sub)(Fmul:=F.mul)(Finv:=F.inv)(Fdiv:=F.div)
+                  (field:=field)(char_ge_3:=char_ge_3)(Feq_dec:=F.eq_dec)
+                  (a:=a)(d:=d)(nonzero_a:=nonzero_a)(a_eq_minus1:=a_eq_minus1)
+                  (twice_d:=twice_d)(k_eq_2d:=k_eq_2d)(nonzero_d:=nonzero_d)). 
+Local Notation multiples :=
+  (multiples(F:=F M_pos)(Feq:=Logic.eq)(Fzero:=F.zero)(Fone:=F.one)
+                  (Fopp:=F.opp)(Fadd:=F.add)(Fsub:=F.sub)(Fmul:=F.mul)(Finv:=F.inv)(Fdiv:=F.div)
+                  (field:=field)(char_ge_3:=char_ge_3)(Feq_dec:=F.eq_dec)
+                  (a:=a)(d:=d)(nonzero_a:=nonzero_a)(a_eq_minus1:=a_eq_minus1)
+                  (twice_d:=twice_d)(k_eq_2d:=k_eq_2d)(square_a:=square_a)(nonsquare_d:=nonsquare_d)). 
+Local Notation scalarmult :=
+  (scalarmult(F:=F M_pos)(Feq:=Logic.eq)(Fzero:=F.zero)(Fone:=F.one)
+                  (Fopp:=F.opp)(Fadd:=F.add)(Fsub:=F.sub)(Fmul:=F.mul)(Finv:=F.inv)(Fdiv:=F.div)
+                  (field:=field)(char_ge_3:=char_ge_3)(Feq_dec:=F.eq_dec)
+                  (a:=a)(d:=d)(nonzero_a:=nonzero_a)(a_eq_minus1:=a_eq_minus1)
+                  (twice_d:=twice_d)(k_eq_2d:=k_eq_2d)(square_a:=square_a)(nonsquare_d:=nonsquare_d)). 
+
+Local Notation "p .+ n" := (word.add p (word.of_Z n)) (at level 50, format "p .+ n", left associativity).
+Local Notation "c 'p5@' p" := (p5at c p) (at level 10, format "c 'p5@' p").
+Local Notation "c 'p4@' p" := (p4at c p) (at level 10, format "c 'p4@' p").
+
+Definition cached_point (p : word) (a : cached) : map.rep -> Prop :=
+  Lift1Prop.ex1 (fun a_repr : cached_repr a => (a_repr p4@ p)).
+Definition projective_point (p : word) (a : point) : map.rep -> Prop :=
+  Lift1Prop.ex1 (fun a_repr : projective_repr a => (a_repr p5@ p)).
+
+Instance spec_of_cached_multiples : spec_of "cached_multiples" :=
+  fnspec! "cached_multiples"
+    (p_ai p_a p_d: word) /
+    (a : point) (a_repr : projective_repr a) (d1: felem) (out : list byte) (R : _ -> Prop), {
+      requires t m :=
+        m =* out $@ p_ai * a_repr p5@ p_a * FElem p_d d1 *  R /\
+        Datatypes.length out = Z.to_nat (16*pc_size) /\
+        d = feval d1 /\
+        bounded_by tight_bounds d1;
+      ensures t' m' :=
+        t = t' /\
+        m' =* (array cached_point (word.of_Z pc_size) p_ai (List.map m1_prep (multiples 16 a))) * a_repr p5@ p_a * FElem p_d d1 * R
+    }.
+
+Local Ltac cbv_bounds H :=
+  cbv [un_xbounds bin_xbounds bin_ybounds un_square bin_mul bin_add bin_carry_add bin_sub bin_carry_sub un_outbounds bin_outbounds] in H;
+  cbv [un_xbounds bin_xbounds bin_ybounds un_square bin_mul bin_add bin_carry_add bin_sub bin_carry_sub un_outbounds bin_outbounds].
+
+Local Ltac solve_bounds :=
+  repeat match goal with
+  | H: bounded_by loose_bounds ?x |- bounded_by loose_bounds ?x => apply H
+  | H: bounded_by tight_bounds ?x |- bounded_by tight_bounds ?x => apply H
+  | H: bounded_by tight_bounds ?x |- bounded_by loose_bounds ?x => apply relax_bounds
+  | H: bounded_by _ ?x |- bounded_by _ ?x => cbv_bounds H
+  end.
+
+Ltac skipn_firstn_length :=
+  change felem_size_in_bytes with 40 in *; listZnWords.
+
+Ltac split_stack_at_n_in stack p n H := rewrite <- (firstn_skipn n stack) in H;
+  rewrite (map.of_list_word_at_app_n _ _ _ n) in H; try skipn_firstn_length;
+  let D := fresh in unshelve(epose (sep_eq_putmany _ _ (map.adjacent_arrays_disjoint_n p (firstn n stack) (skipn n stack) n _ _)) as D); try skipn_firstn_length;
+  seprewrite_in D H; rewrite ?skipn_skipn in H; bottom_up_simpl_in_hyp H; clear D.
+
+Local Ltac solve_mem :=
+  try match goal with  | |- exists _ : _ -> Prop, _%sep _ => eexists end;
+  match goal with  | H : _ %sep ?m |- _ %sep ?m => bottom_up_simpl_in_goal_nop_ok end;
+  match goal with
+  | |- _%sep _ => ecancel_assumption_impl
+  | H: ?P%sep ?m |- ?G%sep ?m =>  (* Solve Placeholder goals when a fixed size list is given *)
+    match P with context[map.of_list_word_at ?p ?stack] =>
+    match G with context[Placeholder ?p _] =>
+      solve [ cbv [Placeholder]; extract_ex1_and_emp_in_goal; bottom_up_simpl_in_goal_nop_ok; split; [ecancel_assumption | skipn_firstn_length] ]
+    end end
+  end.
+
+Local Ltac single_step :=
+  repeat straightline; straightline_call; ssplit; try solve_mem; try solve_bounds;
+  (* solve simple preconditions *) try listZnWords; try assumption.
+
+Local Instance spec_of_zero_projective_point: spec_of "zero_projective_point" := spec_of_zero_projective_point (a:=a) (d:=d) (nonzero_a:=nonzero_a).
+Local Instance spec_of_to_cached : spec_of "to_cached" := spec_of_to_cached (nonzero_d:=nonzero_d) (k_eq_2d:=k_eq_2d) (twice_d:=twice_d) (a_eq_minus1:=a_eq_minus1) (nonzero_a:=nonzero_a) (d:=d) (a:=a).
+Local Instance spec_of_copy_projective_point : spec_of "copy_projective_point" := spec_of_copy_projective_point (a:=a) (d:=d).
+Local Instance spec_of_double : spec_of "double" := spec_of_double (k_eq_2d:=k_eq_2d) (a_eq_minus1:=a_eq_minus1) (nonsquare_d:=nonsquare_d) (square_a:=square_a) (nonzero_a:=nonzero_a) (a:=a) (d:=d) (twice_d:=twice_d).
+Local Instance spec_of_of_readd : spec_of "readd" := spec_of_readd (nonzero_d:=nonzero_d) (k_eq_2d:=k_eq_2d) (twice_d:=twice_d) (a_eq_minus1:=a_eq_minus1) (nonsquare_d:=nonsquare_d) (square_a:=square_a) (nonzero_a:=nonzero_a) (d:=d) (a:=a).
+
+Lemma cached_multiples_ok: program_logic_goal_for_function! cached_multiples.
+Proof.
+   (* Without this, resolution of cbv stalls out Qed. *)
+   (* TODO can't I mark these as opaque in this section and the locally, in a tactic unopaque them when needed. (Or opaque below, where the actual harm happens, which is probably modulo arithmetics.)*)
+  Strategy -1000 [un_xbounds bin_xbounds bin_ybounds un_square bin_mul bin_add bin_carry_add bin_sub bin_carry_sub un_outbounds bin_outbounds].
+
+
+  (* put zero into ai[0] *)
+  repeat straightline.
+  seprewrite_in array1_iff_eq_of_list_word_at H9; [lia|].
+  single_step.
+  repeat straightline.
+  split_stack_at_n_in out p_ai 160%nat H21. (* split out ai[0] *)
+  single_step.
+  
+  (* put A into ai[1] *)
+  repeat straightline.
+  split_stack_at_n_in (skipn 160 out) (p_ai.+160) 160%nat H22. (* split out ai[1]*)
+  single_step.
+
+  (* allocate helper array (and split it up here already? might make stuff slow) *)
+  repeat straightline.
+  seprewrite_in array1_iff_eq_of_list_word_at H23; [lia|]. (* because allocation uses array, best way is to build a switch for allocation to use $@. *)
+
+  (* copy over 1*A to p_ai_uncached *)
+  split_stack_at_n_in stack1 a4 200%nat H23. (* index 0 - unused*)
+  split_stack_at_n_in (skipn 200 stack1) (a4.+200) 200%nat H23. (* index 1, will now be filled *)
+  single_step.
+  repeat straightline. 
+
+  (* Loop! *)
+  refine (let multiples_a := multiples 16 a0 in
+          let cached_multiples_a := List.map m1_prep multiples_a in
+          let uncached_multiples_a := List.firstn 8 multiples_a in
+          tailrec
+            (* I think R may change, so it'd be nice to have here, let's see.  *)
+            (HList.polymorphic_list.cons (_(*temp_value*)) HList.polymorphic_list.nil)
+            (*variables*)(["temp"; "i"; "p_ai_uncached"; "zero"; "p_a"; "p_d"; "p_ai"]) (* these must be all variables we have, even if we don't use them*)
+            (*spec*)(fun v temp_value t m temp i p_ai_uncached zero p_a p_d p_ai=>
+                let i_z := word.unsigned i in
+                PrimitivePair.pair.mk
+                  (* Invariant *)
+                  (v = (8 - i_z / 2) /\
+                   i_z mod 2 = 0 /\ 2 <= i_z < 16 /\
+                   m =* 
+                        (* p_ai contains 0 - (i-1) of cached_multiples *)
+                        array cached_point (word.of_Z pc_size) p_ai (List.firstn (Z.to_nat (i_z)) cached_multiples_a) *
+                        (* the remaining space of p_ai is unused*)
+                        (skipn (Z.to_nat ((i_z) * pc_size)) out) $@ (p_ai .+ ((i_z) * pc_size)) *
+                        (* p_ai_uncached contains 0 - (i-1) of uncached_multiples, maximum 0-7 *)
+                        array projective_point (word.of_Z pp_size)
+                          p_ai_uncached (List.firstn (Z.to_nat (i_z)) uncached_multiples_a) *
+                        (* and (if there is any), the rest of its memory is unused *)
+                        (skipn (Z.to_nat ((i_z) * pp_size)) stack1) $@ (p_ai_uncached .+ ((i_z) * pp_size)) *
+                        (* temp can be anything, it's only used within the loop *)
+                        temp_value $@ temp *
+                        (* remaining memory is left untouched *)
+                        a_repr p5@ p_a * FElem p_d d1 * R /\
+                        Datatypes.length temp_value = Z.to_nat pp_size)
+                  (* Postcondition Schema *)
+                  (fun T_f M_f temp_f i_f p_ai_uncached_f zero_f p_a_f p_d_f p_ai_f =>
+                     T_f = t /\ 
+                     M_f =* array cached_point (word.of_Z pc_size) p_ai cached_multiples_a *
+                            a_repr p5@ p_a * FElem p_d d1 * R)) (* hmmm, actually there's some more stuff in memory, right? I probably need that*)
+            (*measure*)(fun n m : Z => 0 <= n < m) _ _ _ _ _ _); loop_simpl.
+
+  { repeat straightline. }
+  { exact (Z.lt_wf _). }
+  {
+    repeat straightline.
+    ssplit; try ZnWords. 
+    (* Memory precondition, the first two are filled. Actually they are not because I left out zero, probably should just shift the array by one - fix later and look at the body first. *)
+    admit. admit.
+  }
+  {
+    repeat straightline.
+    (* Single out i/2 * A from uncached multiples. *)
+    replace ((firstn (Z.to_nat (word.unsigned x4)) uncached_multiples_a)) with
+            ((firstn (Z.to_nat (word.unsigned x4 /2)) (firstn (Z.to_nat (word.unsigned x4)) uncached_multiples_a)) ++ 
+            (scalarmult (Z.to_nat (word.unsigned x4 /2)) a0) :: 
+            (skipn (S(Z.to_nat (word.unsigned x4 /2))) (firstn (Z.to_nat (word.unsigned x4)) uncached_multiples_a)))%list
+            in H36.
+    2: {
+      clear - H35 H38 H34.
+      rewrite firstn_skipn_middle.
+      2:{ cbv delta [uncached_multiples_a multiples_a]. erewrite nth_error_nth'. cbv delta [uncached_multiples_a multiples_a]. rewrite !firstn_multiples. rewrite multiples_correct. reflexivity. Lia.lia. rewrite !firstn_length, length_multiples. Lia.lia.  }
+      reflexivity.
+    }
+    rewrite !array_app in H36. rewrite array_cons in H36 (* this crashes for some reason. fix next. *). unfold array at 3 in H36.
+
+    replace (x5.+200 *Z.of_nat (Datatypes.length (firstn (Z.to_nat (word.unsigned x4 / 2)) (firstn (Z.to_nat (word.unsigned x4)) uncached_multiples_a)))) with
+      ((word.add x5 (word.mul (word.sru x4 (word.of_Z 1)) (word.of_Z 200)))) in H36.
+    cbv [projective_point] in H36. extract_ex1_and_emp_in H36.
+
+    (* Double (i/2)*A -> temp contains i*A.  *)
+    single_step.
+    repeat straightline.
+    
+    (* split out ai[i]*)
+    split_stack_at_n_in (skipn (Z.to_nat (word.unsigned x4 * 160)) out) (x9.+word.unsigned x4 * 160) 160%nat H41. 
+    (* copy temp into ai[i] *)
+    single_step.
+
+    repeat straightline. (* why doesn't straightline work with my if? *)
+    (* if condition and saving into p_ai_uncached is next. *)
+    unfold1_cmd_goal; cbv beta match delta [cmd_body].
+    repeat straightline.
+    split. (* if cases - this may get weird cause the rest doesn't depend on the if... *)
+
+    (*  i < 8 -> copy i*A into p_ai_uncached *)
+    single_step.
+    (* oh wait, wrong assumption *)
+
+    Admitted.
+
+End WithParameters.
